pulse/lib/steel/pulse/Pulse.Checker.Bind.fst
@@ -137,9 +137,9 @@ let bind_res_and_post_typing (g:env) (s2:st_comp) (x:var { Metatheory.fresh_wrt 
       (* since we need to type the result in a smaller env g *)          
       let (| u, res_typing |) = check_universe g s2.res in 
       if not (eq_univ u s2.u)
-      then T.fail "Unexpected universe for result type"
+      then fail g None "Unexpected universe for result type"
       else if x `Set.mem` freevars s2.post
-      then T.fail (Printf.sprintf "Bound variable %d escapes scope in postcondition %s" x (P.term_to_string s2.post))
+      then fail g None (Printf.sprintf "Bound variable %d escapes scope in postcondition %s" x (P.term_to_string s2.post))
       else (
         let y = x in //fresh g in
         let s2_post_opened = open_term_nv s2.post (v_as_nv y) in
@@ -148,7 +148,7 @@ let bind_res_and_post_typing (g:env) (s2:st_comp) (x:var { Metatheory.fresh_wrt 
       )
     | Some post -> 
       if x `Set.mem` freevars s2.post
-      then T.fail "Unexpected mismatched postcondition in bind" //exclude with a stronger type on check'
+      then fail g None "Unexpected mismatched postcondition in bind" //exclude with a stronger type on check'
       else (
          let pr = Pulse.Checker.Common.post_hint_typing g post x in
          pr.ty_typing, pr.post_typing
@@ -176,7 +176,7 @@ let  mk_bind' (g:env)
    =  let _,x  = px in
       let s2 = st_comp_of_comp c2 in
       if x `Set.mem` freevars s2.post
-      then T.fail (Printf.sprintf "Bound variable %d escapes scope in postcondition %s" x (P.term_to_string s2.post))
+      then fail g None (Printf.sprintf "Bound variable %d escapes scope in postcondition %s" x (P.term_to_string s2.post))
       else ( 
         let res_typing, post_typing = bind_res_and_post_typing g s2 x post_hint  in
         let (| t, c, d |) = mk_bind g pre e1 e2 c1 c2 px d_e1 d_c1res d_e2 res_typing post_typing in
@@ -198,7 +198,7 @@ let check_bind
   let Tm_Bind { binder=b; head=e1; body=e2 } = t.term in
   let (| e1, c1, d1 |) = check g e1 pre pre_typing None in
   if not (stateful_comp c1)
-  then T.fail "Bind: c1 is not st"
+  then fail g None "Bind: c1 is not st"
   else 
     let s1 = st_comp_of_comp c1 in
     let t = s1.res in
@@ -210,7 +210,7 @@ let check_bind
     let (| e2', c2, d2 |) = check g' (open_st_term_nv e2 px) next_pre next_pre_typing post_hint in
     FV.st_typing_freevars d2;
     if not (stateful_comp c2)
-    then T.fail "Bind: c2 is not st"
+    then fail g None "Bind: c2 is not st"
     else ( 
       let e2_closed = close_st_term e2' x in
       assume (open_st_term e2_closed x == e2');
@@ -240,7 +240,7 @@ let check_tot_bind g t pre pre_typing post_hint check =
   let (| e2, c2, e2_typing |) =
     check g' (open_st_term_nv e2 px) pre pre_typing' post_hint in
   if not (stateful_comp c2)
-  then T.fail "Tm_TotBind: e2 is not a stateful computation"
+  then fail g (Some e2.range) "Tm_TotBind: e2 is not a stateful computation"
   else
     let e2_closed = close_st_term e2 x in
     assume (open_st_term_nv e2_closed (v_as_nv x) == e2);
