pulse/lib/steel/pulse/Pulse.Checker.If.fst
@@ -27,7 +27,7 @@ let rec combine_if_branches
            (requires fun _ ->
               comp_pre c_then == comp_pre c_else)
            (ensures fun _ _ -> True) =
-
+  let g = g_then in
   if eq_st_comp (st_comp_of_comp c_then) (st_comp_of_comp c_else)
   then begin
     match c_then, c_else with
@@ -36,7 +36,7 @@ let rec combine_if_branches
     | C_STGhost inames1 _, C_STGhost inames2 _ ->
       if eq_tm inames1 inames2
       then (| c_then, e_then_typing, e_else_typing |)
-      else T.fail "Cannot combine then and else branches (different inames)"
+      else fail g None "Cannot combine then and else branches (different inames)"
     | C_ST _, C_STAtomic inames _ ->
       if eq_tm inames Tm_EmpInames
       then begin
@@ -45,7 +45,7 @@ let rec combine_if_branches
             (Lift_STAtomic_ST g_else c_else) in
         (| c_then, e_then_typing, e_else_typing |)
       end
-      else T.fail "Cannot lift STAtomic else branch to match then"
+      else fail g None "Cannot lift STAtomic else branch to match then"
     | C_STAtomic inames _, C_ST _ ->
       if eq_tm inames Tm_EmpInames
       then begin
@@ -54,7 +54,7 @@ let rec combine_if_branches
             (Lift_STAtomic_ST g_then c_then) in
         (| c_else, e_then_typing, e_else_typing |)
       end
-      else T.fail "Cannot lift STAtomic else branch to match then"
+      else fail g None "Cannot lift STAtomic else branch to match then"
     | C_STGhost _ _, _ ->
       let w = get_non_informative_witness g_then (comp_u c_then) (comp_res c_then) in
       let e_then_typing =
@@ -67,9 +67,9 @@ let rec combine_if_branches
       let e_else_typing =
         T_Lift _ _ _ _ e_else_typing (Lift_STGhost_STAtomic _ _ w) in
       combine_if_branches _ _ _ e_then_typing _ _ _ e_else_typing
-    | _, _ -> T.fail "Cannot combine then and else branches (incompatible effects)"
+    | _, _ -> fail g None "Cannot combine then and else branches (incompatible effects)"
   end
-  else T.fail "Cannot combine then and else branches (different st_comp)"
+  else fail g None "Cannot combine then and else branches (different st_comp)"
 #pop-options
 
 #push-options "--query_stats --ifuel 2 --z3rlimit_factor 4"
@@ -102,9 +102,9 @@ let check_if (g:env)
             check g_with_eq br pre pre_typing (Some post_hint)
         in
         if hyp `Set.mem` freevars_st br
-        then T.fail "Illegal use of control-flow hypothesis in branch"
+        then fail g (Some br.range) "Illegal use of control-flow hypothesis in branch"
         else if not (stateful_comp c)
-        then T.fail "Branch computation type not st"
+        then fail g (Some br.range) "Branch computation type not st"
         else (| br, c, br_typing |)
     in 
     let (| e1, c1, e1_typing |) = check_branch tm_true e1 in
@@ -114,12 +114,12 @@ let check_if (g:env)
     let c_typing = 
       let x = fresh g in
       if x `Set.mem` freevars post //exclude this
-      then T.fail "Unexpected name clash"
+      then fail g None "Unexpected name clash"
       else if not (eq_tm (comp_res c) post_hint.ret_ty &&
                    eq_univ (comp_u c) post_hint.u &&
                    eq_tm (comp_post c) post_hint.post) //exclude by check' strengthening
       then (
-        T.fail "Unexpected result type in branches"
+        fail g None "Unexpected result type in branches"
       )
       else (
         let post_typing = post_hint_typing g post_hint x in
