pulse/lib/steel/pulse/Pulse.Checker.Inference.fst
@@ -55,7 +55,7 @@ let gen_uvar (name:ppname) =
   let nm = T.unseal name.name in
   (n, name), wrap_nat_to_uvar nm name.range n
 
-let rec gen_uvars (t_head:term) : T.Tac (list uvar & comp) =
+let rec gen_uvars (g:env) (t_head:term) : T.Tac (list uvar & comp) =
   let ropt = is_arrow t_head in
   match ropt with
   | Some (b, Some Implicit, c_rest) -> (
@@ -67,14 +67,14 @@ let rec gen_uvars (t_head:term) : T.Tac (list uvar & comp) =
     | C_STGhost _ c ->
       [n], c_rest
     | C_Tot t ->
-      let n_rest, comp_typ = gen_uvars t in
+      let n_rest, comp_typ = gen_uvars g t in
       n::n_rest, comp_typ
   )
   | _ ->
-   T.fail (FStar.Printf.sprintf "gen_uvars: unexpected t_head: %s"
+   fail g None (FStar.Printf.sprintf "gen_uvars: unexpected t_head: %s"
                                   (P.term_to_string t_head))
 
-let rec check_valid_solution (n:uvar) (t:term) (uv_sols:solution)
+let rec check_valid_solution (g:env) (n:uvar) (t:term) (uv_sols:solution)
   : T.Tac solution =
 
   match uv_sols with
@@ -82,8 +82,8 @@ let rec check_valid_solution (n:uvar) (t:term) (uv_sols:solution)
   | (n', t')::tl ->
     if uvar_eq n n'
     then if eq_tm t t' then uv_sols
-         else T.fail "check_valid_solution failed"
-    else (n', t')::(check_valid_solution n t tl)
+         else fail g None "check_valid_solution failed"
+    else (n', t')::(check_valid_solution g n t tl)
 
 let uvar_index (t:term{Some? (is_uvar t)}) : uvar =
   Some?.v (is_uvar t)
@@ -112,27 +112,27 @@ let is_reveal (t:term) : bool =
      | _ -> false)
   | _ -> false
 
-let rec match_typ (t1 t2:term) (uv_sols:solution)
+let rec match_typ (g:env) (t1 t2:term) (uv_sols:solution)
   : T.Tac solution =
 
   match is_reveal_uvar t1, is_reveal t2 with
   | Some (u, ty, t), false ->
-    check_valid_solution (uvar_index t) (mk_hide u ty t2) uv_sols
+    check_valid_solution g (uvar_index t) (mk_hide u ty t2) uv_sols
   | _ ->
     if Some? (is_uvar t1)
-    then check_valid_solution (uvar_index t1) t2 uv_sols
+    then check_valid_solution g (uvar_index t1) t2 uv_sols
     else if Some? (is_uvar t2)
-    then T.fail "match_typ: t2 is a uvar"
+    then fail g None "match_typ: t2 is a uvar"
     else match t1, t2 with
          | Tm_Pure t1, Tm_Pure t2 ->
-           match_typ t1 t2 uv_sols
+           match_typ g t1 t2 uv_sols
     
          | _, _ ->
            match is_pure_app t1, is_pure_app t2 with
            | Some (head1, arg_qual1, arg1), Some (head2, arg_qual2, arg2) ->
              if arg_qual1 = arg_qual2
-             then let uv_sols = match_typ head1 head2 uv_sols in
-                  match_typ arg1 arg2 uv_sols
+             then let uv_sols = match_typ g head1 head2 uv_sols in
+                  match_typ g arg1 arg2 uv_sols
              else uv_sols
 
            | _, _ -> uv_sols
@@ -166,7 +166,7 @@ let rec atomic_vprops_may_match (t1:term) (t2:term) : bool =
            atomic_vprops_may_match arg1 arg2
          | _, _ -> eq_tm t1 t2
 
-let infer_one_atomic_vprop (t:term) (ctxt:list term) (uv_sols:solution)
+let infer_one_atomic_vprop (g:env) (t:term) (ctxt:list term) (uv_sols:solution)
   : T.Tac solution =
 
   if atomic_vprop_has_uvar t
@@ -181,7 +181,7 @@ let infer_one_atomic_vprop (t:term) (ctxt:list term) (uv_sols:solution)
       //                    (P.term_to_string t)
       //                    (P.term_to_string (List.Tot.hd matching_ctxt))
       //                    (List.Tot.length uv_sols)) in 
-      let uv_sols = match_typ t (List.Tot.hd matching_ctxt) uv_sols in
+      let uv_sols = match_typ g t (List.Tot.hd matching_ctxt) uv_sols in
       // T.print (FStar.Printf.sprintf "post matching, uv_sols has %d solutions\n"
       //            (List.Tot.length uv_sols))
       uv_sols
@@ -191,14 +191,15 @@ let infer_one_atomic_vprop (t:term) (ctxt:list term) (uv_sols:solution)
 let union_ranges (r0 r1:range) : T.Tac range = r0
 let with_range (t:st_term') (r:range) : st_term = { term = t; range = r}
 
-let rec rebuild_head (head:term) (uvs:list uvar) (uv_sols:solution) (r:range)
+let rec rebuild_head (g:env) (head:term) (uvs:list uvar) (uv_sols:solution) (r:range)
   : T.TacH st_term (requires fun _ -> List.Tot.length uvs > 0)
                    (ensures fun _ _ -> True) =
   let hd::tl = uvs in
   let ropt = List.Tot.find (fun (n1, _) -> uvar_eq hd n1) uv_sols in
   match ropt with
   | None ->
-    T.fail (FStar.Printf.sprintf
+    fail g (Some r)
+           (FStar.Printf.sprintf
               "inference failed in building head, no solution for %s\n"
               (uvar_to_string hd))
   | Some (_, t2) ->
@@ -207,7 +208,7 @@ let rec rebuild_head (head:term) (uvs:list uvar) (uv_sols:solution) (r:range)
                        r
     | _ ->
       let app_node = tm_pureapp head (Some Implicit) t2 in
-      rebuild_head app_node tl uv_sols r
+      rebuild_head g app_node tl uv_sols r
 
 
 let print_solutions (l:solution)
@@ -229,7 +230,7 @@ let find_solution (sol:solution) (t:uvar)
     | Some (_, t) -> Some t
 
 
-let try_inst_uvs_in_goal (ctxt:term)
+let try_inst_uvs_in_goal (g:env) (ctxt:term)
                          (goal:vprop)
   : T.Tac solution
   = let uv_sols = [] in
@@ -238,7 +239,7 @@ let try_inst_uvs_in_goal (ctxt:term)
     let uv_sols =
       T.fold_left
         (fun uv_sols goal_vprop ->
-          infer_one_atomic_vprop goal_vprop ctxt_list uv_sols)
+          infer_one_atomic_vprop g goal_vprop ctxt_list uv_sols)
         uv_sols
         goal_list
     in
@@ -248,23 +249,24 @@ let try_inst_uvs_in_goal (ctxt:term)
 
 
 let infer
+  (g:env)
   (head:term)
   (t_head:term)
   (ctxt_pre:term)
   (r:range)
   : T.Tac st_term =
-
+  let g = push_context g "infer" r in
   let uvs, pre =
-    let uvs, comp = gen_uvars t_head in
+    let uvs, comp = gen_uvars g t_head in
     match comp with
     | C_ST st_comp
     | C_STAtomic _ st_comp
     | C_STGhost _ st_comp -> uvs, st_comp.pre
-    | _ -> T.fail "infer:unexpected comp type"
+    | _ -> fail g (Some r) "infer:unexpected comp type"
   in
 
   if List.Tot.length uvs = 0
-  then T.fail "Inference did not find anything to infer"
+  then fail g (Some r) "Inference did not find anything to infer"
   else begin
     // T.print (FStar.Printf.sprintf "infer: generated %d uvars,\n\
     //                                ctx: {\n%s\n}\n\
@@ -272,9 +274,9 @@ let infer
     //            (List.Tot.length uvs)
     //            (P.term_list_to_string "\n" (vprop_as_list ctxt_pre))
     //            (P.term_list_to_string "\n" (vprop_as_list pre)));
-    let uv_sols = try_inst_uvs_in_goal ctxt_pre pre in
+    let uv_sols = try_inst_uvs_in_goal g ctxt_pre pre in
     // T.print (Printf.sprintf "Got solutions: {\n%s\}"  (print_solutions uv_sols));
-    let head = rebuild_head head uvs uv_sols r in
+    let head = rebuild_head g head uvs uv_sols r in
     // T.print (Printf.sprintf "Rebuilt head= %s" (P.st_term_to_string head));
     head
   end
@@ -371,7 +373,7 @@ let rec contains_uvar (t:term)
     | Tm_FStar t _ ->
       contains_uvar_r t
 
-let try_unify (l r:term) = match_typ l r []
+let try_unify (g:env) (l r:term) = match_typ g l r []
 
 module RF = FStar.Reflection.Formula
 
@@ -387,7 +389,7 @@ let is_eq2 (t:R.term) : option (R.term & R.term) =
     else None
   | _ -> None
 
-let try_solve_pure_equalities (p:term) : T.Tac solution =
+let try_solve_pure_equalities (g:env) (p:term) : T.Tac solution =
   let rec aux (sol:solution) (t:R.term) : T.Tac solution =
     let open RF in
     let t = apply_sol sol t in
@@ -397,7 +399,7 @@ let try_solve_pure_equalities (p:term) : T.Tac solution =
       || contains_uvar_r t1
       then (
         assume (not_tv_unknown t0 /\ not_tv_unknown t1);
-        try_unify (Tm_FStar t0 FStar.Range.range_0) (Tm_FStar t1 FStar.Range.range_0) @ sol
+        try_unify g (Tm_FStar t0 FStar.Range.range_0) (Tm_FStar t1 FStar.Range.range_0) @ sol
       )
       else sol
     in
